# ðŸ“• Solution

```java
import java.io.BufferedReader;
import java.io.BufferedWriter;
import java.io.IOException;
import java.io.InputStreamReader;
import java.io.OutputStreamWriter;

class Main {
    public static final long REMAIN = 1000000007;
    public static long[][] Multiplicative(long[][] a, long[][] b){
        long[][] temp = {{0, 0}, {0, 0}};
        for(int i = 0; i < 2; i++){
            for(int j = 0; j < 2; j++){
                for(int k = 0; k < 2; k++) {
                    temp[i][j] += (a[i][k] * b[k][j]) % REMAIN;
                }
                temp[i][j] %= REMAIN;
            }
        }
        return temp;
    }
    public static long[][] Count(long[][] arr, long n){
        if(n == 1L){
            return arr;
        }
        long[][] temp = Count(arr, n / 2);
        if(n % 2 == 0){
            return Multiplicative(temp, temp);
        } else {
            return Multiplicative(Multiplicative(temp, temp), arr);
        }
    }
    public static void main(String[] args) throws IOException {
        BufferedReader br = new BufferedReader(new InputStreamReader(System.in));
        BufferedWriter bw = new BufferedWriter(new OutputStreamWriter(System.out));
        long n = Long.parseLong(br.readLine());
        long[][] arr = {{1, 1}, {1, 0}};
        long[][] answer = Count(arr, n);
        bw.write(answer[0][1] + "");
        br.close();
        bw.close();
    }
}
```

## âŒ fail

```java

```

## ðŸ“‘ Memo

F(2 * n - 1) = F(n) * F(n) + F(n - 1) * F(n - 1)

F(2 * n) = (F(n - 1) + F(n + 1)) * F(n) = (2 * F(n - 1) + F(n)) * F(n)

ë‚˜ëˆ„ëŠ” ê°’ì´ 10^k ì¼ ë•Œ, ì£¼ê¸°ëŠ” 15 * 10 ^ (k - 1) ìž…ë‹ˆë‹¤.
